AP.lean
@@ -3,13 +3,5 @@ import Mathlib.Tactic
 import AP.System.Main
 import AP.Sokoban.Main
 
-def mp₁ : Map ℕ String :=
-  .ofList [(5, "x"), (7, "y")]
-
-def mp₂ : Map ℕ String :=
-  .ofList [(7, "y"), (5, "x")]
-
 def main : IO Unit := do
-  IO.println # mp₁.toList
-  IO.println # mp₂.toList
-  IO.println # decide # mp₁ = mp₂
+  IO.println "ok"
