AP/Util/Basic.lean
@@ -7,6 +7,7 @@ import AP.Util.Sigma
 import AP.Util.Order
 import AP.Util.Option
 import AP.Util.Fintype
+import AP.Util.Algebra
 import AP.Util.Quotient
 import AP.Util.Multiset
 import AP.Util.SetTheory
