AP/Util/Data/Raw/RawChange.lean
@@ -1,0 +1,4 @@
+import AP.Util.Data.Raw.RawData
+
+inductive RawChange where
+| exact : RawData → RawChange
