AP/Util/Logic.lean
@@ -160,3 +160,7 @@ r a b ↔ r c d := by
     apply hr.symm; exact h₂
 
 theorem not_and_iff_or {P Q} : ¬(P ∧ Q) ↔ ¬P ∨ ¬Q := by tauto
+
+theorem ne_symm' {α : Type*} {a b : α} (h : ¬(a = b)) : ¬(b = a) := by tauto
+
+theorem ne_comm' {α : Type*} {a b : α} : ¬(a = b) ↔ ¬(b = a) := by tauto
